theories/SubstExec.v
@@ -9,6 +9,7 @@ License: CC-by 4.0.
 
 Set Implicit Arguments.
 From Sep Require Import Semantics.
+Import LibListExec.RewListExec.
 Open Scope string_scope.
 
 (** [subst_exec] is like [subst] except that it computes with [simpl]. *)
@@ -24,18 +25,18 @@ Fixpoint subst_exec (y:var) (w:val) (t:trm) : trm :=
   let aux_no_capture z t :=
     bind_no_capture z t (aux t) in
   let aux_no_captures xs t :=
-    if mem_exec var_eq y xs then t else aux t in
+    if LibListExec.mem var_eq y xs then t else aux t in
   match t with
   | trm_val v => trm_val v
   | trm_var x => if var_eq x y then trm_val w else t
   | trm_fixs f xs t1 => trm_fixs f xs (bind_no_capture f t1 (aux_no_captures xs t1))
-  | trm_constr id ts => trm_constr id (List.map aux ts)
+  | trm_constr id ts => trm_constr id (LibListExec.map aux ts)
   | trm_if t0 t1 t2 => trm_if (aux t0) (aux t1) (aux t2)
   | trm_let z t1 t2 => trm_let z (aux t1) (aux_no_capture z t2)
-  | trm_apps t0 ts => trm_apps (aux t0) (List.map aux ts)
+  | trm_apps t0 ts => trm_apps (aux t0) (LibListExec.map aux ts)
   | trm_while t1 t2 => trm_while (aux t1) (aux t2)
   | trm_for x t1 t2 t3 => trm_for x (aux t1) (aux t2) (aux_no_capture x t3)
-  | trm_match t0 pts => trm_match (aux t0) (List.map (fun '(pi,ti) =>
+  | trm_match t0 pts => trm_match (aux t0) (LibListExec.map (fun '(pi,ti) =>
        (pi, aux_no_captures (patvars pi) ti)) pts)
   | trm_fail => trm_fail
   end.
@@ -43,16 +44,19 @@ Fixpoint subst_exec (y:var) (w:val) (t:trm) : trm :=
 (** Proof of equivalence between [subst_exec] and [subst].
     First, a few auxiliary lemmas. Then, then induction. *)
 
+Definition eq_exec A (cmp:A->A->bool) : Prop :=
+  forall x y, cmp x y = isTrue (x = y).
+
 Lemma eq_exec_var_eq : eq_exec var_eq.
 Proof using. intros x y. rewrite~ var_eq_spec. Qed.
 
 Lemma if_var_eq_spec : forall x y A (X Y:A),
   (if var_eq x y then X else Y) = (If x = y then X else Y).
-Proof using. intros. rewrite var_eq_spec, if_classicT_eq_if_isTrue. auto. Qed.
+Proof using. intros. rewrite var_eq_spec. rewrite <- if_isTrue. auto. Qed.
 
 Lemma mem_exec_var_eq_eq : forall y xs,
-  mem_exec var_eq y xs = isTrue (mem y xs).
-Proof using. intros. applys mem_exec_eq. applys eq_exec_var_eq. Qed.
+  LibListExec.mem var_eq y xs = isTrue (mem y xs).
+Proof using. intros. applys LibListExec.mem_exec_eq. applys eq_exec_var_eq. Qed.
 
 Lemma subst_exec_eq_subst :
   subst_exec = subst.
@@ -61,11 +65,11 @@ Proof using.
   { rewrite~ if_var_eq_spec. }
   { rewrite mem_exec_var_eq_eq. destruct b; [|try rewrite if_var_eq_spec];
     repeat case_if; tryfalse; auto. }
-  { rewrite List_map_eq. applys* map_congr. }
+  { rew_list_exec. applys* map_congr. }
   { destruct b; [|try rewrite if_var_eq_spec];
     repeat case_if; tryfalse; auto. }
-  { rewrite List_map_eq. applys~ map_congr. }
+  { rew_list_exec. applys~ map_congr. }
   { rewrite if_var_eq_spec. repeat case_if; auto. }
-  { rewrite List_map_eq. applys map_congr. intros (pi,ti) Mi. fequals.
-    rewrite mem_exec_var_eq_eq. rewrite if_classicT_eq_if_isTrue. case_if*. }
+  { rew_list_exec. applys map_congr. intros (pi,ti) Mi. fequals.
+    rewrite mem_exec_var_eq_eq. rewrite <- if_isTrue. case_if*. }
 Qed.
