theories/SLFLift.v
@@ -4,6 +4,13 @@ Foundations of Separation Logic
 
 Chapter: "Lift".
 
+Author: Arthur Charguéraud.
+License: CC-by 4.0.
+
+*)
+
+(*
+
 This chapter describes the "lifting" technique that enables smoother
 specification in a Separation Logic (shallowly) embeded in the proof
 assistant logic. The idea is to relate program values with corresponding
@@ -11,13 +18,7 @@ logical values, e.g. a program boolean with a logical boolean.
 This relation is exploited to more concisely specify return values and
 values that are stored in the heap.
 
-Author: Arthur Charguéraud.
-License: CC-by 4.0.
-
 *)
-
-
-(*
 
 
 
